formatting

theories/models/delaystate_model.v
@@ -1,3 +1,5 @@
+(* monae: Monadic equational reasoning in Coq                                 *)
+(* Copyright (C) 2025 monae authors, license: LGPL-2.1-or-later               *)
 Require Import JMeq.
 From mathcomp Require Import all_ssreflect.
 From mathcomp Require boolp.
@@ -5,6 +7,9 @@ From HB Require Import structures.
 Require Import hierarchy monad_lib fail_lib state_lib trace_lib.
 Require Import monad_transformer.
 
+(**md**************************************************************************)
+(* # Combination of the Delay monad with the state monad transformer          *)
+(******************************************************************************)
 
 Set Implicit Arguments.
 Unset Strict Implicit.
@@ -14,24 +19,24 @@ Local Open Scope monae_scope.
 
 Module TensorS.
 Section tensors.
-Variable S:UU0.
+Variable S : UU0.
 
 Definition tensorS := fun (A : UU0) => (A * S)%type.
-Definition actmt (X Y : UU0) : (X -> Y) -> tensorS X -> tensorS Y := (fun f : X -> Y =>  (fun xs : X * S => match xs with (x, s) => (f x, s) end)).
+Definition actmt (X Y : UU0) : (X -> Y) -> tensorS X -> tensorS Y :=
+  fun f : X -> Y => fun xs : X * S => match xs with (x, s) => (f x, s) end.
+
 Let tensor_id : FunctorLaws.id actmt.
 Proof.
-rewrite/actmt/FunctorLaws.id => B.
-apply boolp.funext => x.
-by case: x.
+by rewrite/actmt/FunctorLaws.id => B; apply boolp.funext => -[].
 Qed.
+
 Let tensor_o : FunctorLaws.comp actmt.
 Proof.
-rewrite/actmt/FunctorLaws.comp => X Y Z g h.
-apply boolp.funext => x.
-by case: x.
+by rewrite/actmt/FunctorLaws.comp => X Y Z g h; apply boolp.funext => -[].
 Qed.
 
 HB.instance Definition _:= isFunctor.Build tensorS tensor_id tensor_o.
+
 End tensors.
 End TensorS.
 HB.export TensorS.
@@ -40,17 +45,16 @@ Module HomS.
 Section homs.
 Variable S : UU0.
 
-Definition homS := fun (A : UU0) => (S -> A).
-Definition actmh (X Y : UU0) : (X -> Y) -> homS X -> homS Y := fun (f: X -> Y) => fun (m: S ->X) => f \o m.
+Definition homS := fun A : UU0 => S -> A.
+Definition actmh (X Y : UU0) : (X -> Y) -> homS X -> homS Y :=
+  fun f : X -> Y => fun m : S -> X => f \o m.
+
 Let hom_id : FunctorLaws.id actmh.
-Proof.
-rewrite/actmh/FunctorLaws.id => B.
-by apply boolp.funext => x.
-Qed.
+Proof. by rewrite/actmh/FunctorLaws.id => B; exact: boolp.funext. Qed.
+
 Let hom_o : FunctorLaws.comp actmh.
 Proof.
-rewrite/actmh/FunctorLaws.comp => X Y Z g h.
-by apply boolp.funext => x.
+by rewrite/actmh/FunctorLaws.comp => X Y Z g h; exact: boolp.funext.
 Qed.
 
 HB.instance Definition _:= isFunctor.Build homS hom_id hom_o.
@@ -65,15 +69,19 @@ Variable M : delayMonad.
 
 Hint Extern 0 (wBisim _ _) => setoid_reflexivity.
 
-Notation "a '≈' b" := (wBisim a b).
-Notation DS := (MS S M).
+Local Notation "a '≈' b" := (wBisim a b).
+Local Notation DS := (MS S M).
 
-Lemma DSE {X}: DS X  = (homS S \o M \o tensorS S) X.
-Proof. by rewrite/DS/MS/homS/tensorS => //=. Qed.
+Lemma DSE {X} : DS X = (homS S \o M \o tensorS S) X.
+Proof. by []. Qed.
+
 Lemma homSmap {A B} (f : A -> B) (m : S -> A) : (homS S # f) m = f \o m.
 Proof. by []. Qed.
-Lemma tensorSmap {A B} (f : A -> B) (m : tensorS S A) : (tensorS S # f) m = let (a, s) := m in (f a, s).
+
+Lemma tensorSmap {A B} (f : A -> B) (m : tensorS S A) :
+  (tensorS S # f) m = let (a, s) := m in (f a, s).
 Proof. by []. Qed.
+
 Lemma DSmapE {X Y} (f : X -> Y) : DS # f = (homS S \o M \o tensorS S) # f.
 Proof.
 apply boolp.funext => x.
@@ -81,50 +89,53 @@ rewrite -compA FCompE FCompE //= homSmap.
 apply boolp.funext => s //=.
 rewrite fmapE//=/bindS/retS//=/uncurry/curry fmapE/=.
 congr bind.
-apply boolp.funext => xs.
-by case: xs => x' s' //=.
+by apply boolp.funext => -[].
 Qed.
-Definition dist1 {X Y} (s : tensorS S (Y + X)) : (tensorS S Y) + (tensorS S X) :=
-  let (yx, s) := s in match yx with |inl y => inl (y, s) | inr x => inr (x, s) end.
-Definition dist2 {X Y} (xy : (tensorS S Y) + (tensorS  S X)) : tensorS S (Y + X) :=
-  match xy with | inl (y, s) => (inl y, s) | inr (x, s) => (inr x, s) end.
 
-Definition whileDS {X Y} (body : X -> DS (Y + X)) := curry (while (M # dist1 \o uncurry body)).
-Definition wBisimDS A (a b : DS A) := forall s, wBisim (a s) (b s).
+Definition dist1 {X Y} (s : tensorS S (Y + X)) : tensorS S Y + tensorS S X :=
+  let (yx, s) := s in
+  match yx with inl y => inl (y, s) | inr x => inr (x, s) end.
+
+Definition dist2 {X Y} (xy : tensorS S Y + tensorS  S X) : tensorS S (Y + X) :=
+  match xy with inl (y, s) => (inl y, s) | inr (x, s) => (inr x, s) end.
+
+Definition whileDS {X Y} (body : X -> DS (Y + X)) :=
+  curry (while (M # dist1 \o uncurry body)).
+Definition wBisimDS A (a b : DS A) := forall s, a s ≈ b s.
 
 Section wBisimDS.
 Local Notation "a '≈' b" := (wBisimDS a b).
 
 Lemma wBisimDS_refl A (a : DS A) : a ≈ a.
-Proof. move => s. apply wBisim_refl. Qed.
+Proof. by move => s; exact: wBisim_refl. Qed.
 
 Lemma wBisimDS_sym A (d1 d2 : DS A) : d1 ≈ d2 -> d2 ≈ d1.
-Proof. move => Hs s. exact: wBisim_sym. Qed.
+Proof. by move => Hs s; exact: wBisim_sym. Qed.
 
 Lemma wBisimDS_trans A (d1 d2 d3 : DS A) : d1 ≈ d2 -> d2 ≈ d3 -> d1 ≈ d3.
-Proof. move => H1 H2 s. exact/wBisim_trans/H2. Qed.
+Proof. by move => H1 H2 s; exact/wBisim_trans/H2. Qed.
 
 End wBisimDS.
 
-Lemma fixpointDSE {A B} (f : A -> DS (B + A)%type) :
-forall (a : A), wBisimDS (whileDS f a) ( f a >>= (sum_rect (fun => DS B ) Ret (whileDS f))).
+Lemma fixpointDSE {A B} (f : A -> DS (B + A)%type) (a : A) :
+  wBisimDS (whileDS f a) (f a >>= sum_rect (fun => DS B ) Ret (whileDS f)).
 Proof.
-move => a s.
-rewrite/whileDS/curry/dist1/= MS_bindE/uncurry/= fixpointE/= fmapE !bindA.
-apply: bindfwB => bas.
-by case: bas => [[b'|a'] s'] /=; rewrite bindretf.
+move=> s.
+rewrite /whileDS/curry/dist1/= MS_bindE/uncurry/= fixpointE/= fmapE !bindA.
+apply: bindfwB.
+by move=> [[b'|a'] s'] /=; rewrite bindretf.
 Qed.
 
 Lemma naturalityDSE {A B C} (f : A -> DS (B + A)%type) (g : B -> DS C) (a : A) :
-   wBisimDS (bindS (whileDS f a) g) (whileDS (fun y => (f y) >>= (sum_rect (fun => DS (C + A)) (DS # inl \o g) (DS # inr \o (@ret DS A )))) a).
+   wBisimDS (bindS (whileDS f a) g)
+            (whileDS (fun y => f y >>= sum_rect (fun => DS (C + A)) (DS # inl \o g) (DS # inr \o (@ret DS A))) a).
 Proof.
-rewrite/bindS/whileDS/curry/uncurry => s //=.
+rewrite /bindS /whileDS /curry /uncurry => s //=.
 rewrite naturalityE /=.
-apply whilewB => sa.
-case: sa => s' a' /=.
+apply whilewB => -[] s' a' /=.
 rewrite fmapE fmapE /=MS_bindE !bindA.
 apply: bindfwB => sba //=.
-rewrite/dist1/uncurry bindretf.
+rewrite /dist1 /uncurry bindretf.
 case: sba => [[b''|a''] s''] /=.
 - rewrite DSmapE -compA FCompE FCompE homSmap/= fmapE fmapE bindA.
   apply: bindfwB => cs /=.
@@ -137,32 +148,34 @@ case: sba => [[b''|a''] s''] /=.
 Qed.
 
 Lemma codiagonalDSE {A B} (f : A -> DS ((B + A) + A)) (a : A) :
-   wBisimDS (whileDS ((DS # ((sum_rect (fun => (B + A)%type) idfun inr)))  \o f ) a) (whileDS (whileDS f) a).
+   wBisimDS (whileDS ((DS # ((sum_rect (fun => (B + A)%type) idfun inr))) \o f) a)
+            (whileDS (whileDS f) a).
 Proof.
-rewrite/whileDS/curry/wBisimDS => s.
+rewrite /whileDS /curry /wBisimDS => s.
 setoid_symmetry.
 apply: wBisim_trans.
   apply whilewB => sa /=.
   case: sa => s' a' /=.
-  by rewrite /uncurry fmapE naturalityE /=.
+  by rewrite /uncurry fmapE naturalityE.
 rewrite -codiagonalE DSmapE.
-apply whilewB => sa /=.
-case: sa => a'' s'' //=.
-rewrite //=!fmapE.
-have -> : ((homS S \o M) \o tensorS S) # sum_rect (fun=> (B + A)%type) idfun inr = homS S # (M # (tensorS S # sum_rect (fun=> (B + A)%type) idfun inr)).
+apply whilewB => -[] a'' s'' //=.
+rewrite //= !fmapE.
+have -> : ((homS S \o M) \o tensorS S) # sum_rect (fun=> (B + A)%type) idfun inr =
+          homS S # (M # (tensorS S # sum_rect (fun=> (B + A)%type) idfun inr)).
   by rewrite -compA FCompE.
 rewrite homSmap /= fmapE !bindA.
-apply: bindfwB => sbaa.
-by case: sbaa => [[[bl|al']|al] sl]; rewrite !bindretf /= fmapE bindretf /= bindretf.
+apply: bindfwB.
+by move=> [[[bl|al']|al] sl]; rewrite !bindretf /= fmapE bindretf /= bindretf.
 Qed.
 
-Lemma whilewBDS {A B} (f g : A -> DS (B + A)) (a : A) : (forall a, wBisimDS (f a) (g a)) -> wBisimDS (whileDS f a) (whileDS g a).
+Lemma whilewBDS {A B} (f g : A -> DS (B + A)) (a : A) :
+  (forall a, wBisimDS (f a) (g a)) -> wBisimDS (whileDS f a) (whileDS g a).
 Proof.
-rewrite/wBisimDS/whileDS/uncurry/curry => Hfg s.
+rewrite /wBisimDS /whileDS /uncurry /curry => Hfg s.
 apply whilewB => sa /=.
-rewrite! fmapE /=.
+rewrite !fmapE /=.
 case: sa => a'' s'' /=.
-by apply: bindmwB.
+exact: bindmwB.
 Qed.
 
 Lemma bindmwBDS {A B} (f : A -> DS B) (d1 d2 : DS A) :
@@ -177,22 +190,20 @@ by rewrite /wBisimDS => Hfg s /=; rewrite !MS_bindE /=; apply: bindfwB => -[].
 Qed.
 
 Lemma uniformEDS {A B C} (f : A -> DS (B + A)) (g : C -> DS (B + C)) (h : C -> A) :
-  (forall c, f (h c) = g c >>=
-                       sum_rect (fun => DS (B + A))
-                                ((DS # inl) \o Ret)
-                                ((DS # inr) \o Ret \o h)) ->
+  (forall c, f (h c) = g c >>= sum_rect (fun => DS (B + A))
+                                        ((DS # inl) \o Ret)
+                                        ((DS # inr) \o Ret \o h)) ->
   forall c, wBisimDS ((whileDS f) (h c)) (whileDS g c).
 Proof.
 move=> H c s.
 rewrite /whileDS /curry /=.
 set h' := fun (cs : C * S) => let (c, s) := cs in (h c, s).
 have -> : (h c, s) = h' (c, s) by [].
-apply: (uniformE _ _ _ _ _ h') => cs.
-case: cs => [c' s'].
+apply: (uniformE _ _ _ _ _ h') => -[c' s'].
 subst h'.
 rewrite /= fmapE (H c') fmapE /= !bindA.
-apply eq_bind => bcs.
-by case: bcs =>  [[?|?] ?]; rewrite /=bindretf fmapE !bindretf/= fmapE bindretf.
+apply eq_bind.
+by move=> [[?|?] ?]; rewrite /=bindretf fmapE !bindretf/= fmapE bindretf.
 Qed.
 
 HB.instance Definition _ := MonadState.on DS.
