theories/models/delay_monad_model.v
@@ -1,3 +1,5 @@
+(* monae: Monadic equational reasoning in Coq                                 *)
+(* Copyright (C) 2025 monae authors, license: LGPL-2.1-or-later               *)
 From mathcomp Require Import all_ssreflect.
 From mathcomp Require boolp.
 From HB Require Import structures.
